src/Examples/AtomicPair/Helpers.v
@@ -1,0 +1,34 @@
+From iris.algebra Require Import auth.
+Require Export CSL.Refinement ExMach.WeakestPre.
+Unset Implicit Arguments.
+
+(* TODO: move *)
+Section ghost_var_helpers.
+Context {A: ofeT} `{@LeibnizEquiv _ A.(ofe_equiv)} `{OfeDiscrete A}.
+Context {Σ} {Hin: inG Σ (authR (optionUR (exclR A)))}.
+
+Lemma ghost_var_agree γ (a1 a2: A) :
+  own γ (● (Excl' a1)) -∗ own γ (◯ (Excl' a2)) -∗ ⌜ a1 = a2 ⌝.
+Proof.
+  iIntros "Hγ1 Hγ2".
+  iDestruct (own_valid_2 with "Hγ1 Hγ2") as "H".
+  iDestruct "H" as %[<-%Excl_included%leibniz_equiv _]%auth_valid_discrete_2.
+  done.
+Qed.
+
+Lemma ghost_var_update γ (a1' a1 a2 : A) :
+  own γ (● (Excl' a1)) -∗ own γ (◯ (Excl' a2)) ==∗
+    own γ (● (Excl' a1')) ∗ own γ (◯ (Excl' a1')).
+Proof.
+  iIntros "Hγ● Hγ◯".
+  iMod (own_update_2 _ _ _ (● Excl' a1' ⋅ ◯ Excl' a1') with "Hγ● Hγ◯") as "[$$]".
+  { by apply auth_update, option_local_update, exclusive_local_update. }
+  done.
+Qed.
+End ghost_var_helpers.
+
+  (* Extends the iExist tactic to make it easier to re-prove invariants after steps *)
+Instance from_exist_left_sep {Σ} {A} (Φ : A → iProp Σ) Q :
+  FromExist (▷ (∃ a, Φ a) ∗ Q) (λ a, ▷ Φ a ∗ Q)%I .
+Proof. rewrite /FromExist. iIntros "H". iDestruct "H" as (?) "(?&$)". iExists _; eauto. Qed.
+
